Rewrite state_low_projection to obviate functional extensionality.
Rewrite state_low_projection to obviate functional extensionality.

See also discussion in [PR 1685](https://github.com/project-oak/oak/pull/1685) where @jadephilipoom suggested this change.

Like any axiom, functional extensionality can be dangerous to add to a proof, so it is useful to avoid adding it if possible. This change avoids that by writing the low-equivalence relation on the state (and the parts of the state that are functions) so that they are low-equivalent if applying these functions to any argument gives low-equivalent results, rather than defining them in terms of (leibniz) equality directly. 

The proof state is also no worse than it was before.

Co-authored-by: Jade Philipoom <jadep@google.com>

experimental/ni_coq/vfiles/LowEquivalences.v
@@ -47,18 +47,11 @@ Definition node_low_proj := @low_proj node.
 Definition chan_low_proj := @low_proj channel.
 Definition event_low_proj := @low_proj event.
 
-
 Definition node_state_low_proj (ell: level)(ns: node_state): node_state :=
-    fun id => 
-        if (ns id).(lbl) <<? ell 
-            then (ns id)
-            else low_proj ell (ns id).
+    fun id => low_proj ell (ns id).
 
 Definition chan_state_low_proj (ell: level)(cs: chan_state): chan_state :=
-    fun h => 
-        if (cs h).(lbl) <<? ell
-            then (cs h)
-            else low_proj ell (cs h).
+    fun h => low_proj ell (cs h).
 
 Definition state_low_proj (ell: level)(s: state): state := {|
     nodes := node_state_low_proj ell s.(nodes);
@@ -76,12 +69,15 @@ Definition low_eq {A: Type} ell (x: @labeled A) (y: @labeled A) :=
 Definition node_low_eq := @low_eq node.
 Definition chan_low_eq := @low_eq channel.
 Definition event_low_eq := @low_eq event.
-Definition node_state_low_eq := fun ell ns1 ns2 => 
-    (node_state_low_proj ell ns1) = (node_state_low_proj ell ns2).
+Definition node_state_low_eq := fun ell ns1 ns2 =>
+    forall nid, (node_state_low_proj ell ns1) nid = (node_state_low_proj ell ns2) nid.
 Definition chan_state_low_eq := fun ell cs1 cs2 =>
-    (chan_state_low_proj ell cs1) = (chan_state_low_proj ell cs2).
+    forall han, (chan_state_low_proj ell cs1) han = (chan_state_low_proj ell cs2) han.
 Definition state_low_eq := fun ell s1 s2 =>
-    (state_low_proj ell s1) = (state_low_proj ell s2).
+    (forall nid, (state_low_proj ell s1).(nodes) nid =
+        (state_low_proj ell s2).(nodes) nid) /\
+    (forall han, (state_low_proj ell s1).(chans) han=
+        (state_low_proj ell s2).(chans) han ).
 
 (*============================================================================
 * Trace Low Equivalences
